ems/ModSemFacts.v
@@ -18,6 +18,10 @@ Section FACTS.
 Global Program Instance ModSem_OPlusFactsWeak: OPlusFactsWeak (T:=ModSem.t).
 Next Obligation.
   eapply ModSemPair.adequacy.
+  destruct a as [a|]; ss.
+  2: { upt. des_ifs; ss. refl. }
+  destruct b as [b|]; ss.
+  2: { upt. des_ifs; ss. refl. }
   econs.
   { instantiate (1:=top2). ss. }
   2: { instantiate (2:=unit).
@@ -36,6 +40,12 @@ Next Obligation.
 Qed.
 Next Obligation.
   eapply ModSemPair.adequacy.
+  destruct a as [a|]; ss.
+  2: { upt. des_ifs; ss; refl. }
+  destruct b as [b|]; ss.
+  2: { upt. des_ifs; ss; refl. }
+  destruct c as [c|]; ss.
+  2: { upt. des_ifs; ss; refl. }
   econs; eauto.
   { instantiate (1:=top2). ss. }
   2: { instantiate (2:=unit).
@@ -69,13 +79,48 @@ Next Obligation.
   }
 Qed.
 Next Obligation.
-  ii. rr in H. des. rr in H0. des. rr. ss. esplits; et.
+  ii.
+  upt. des_ifs.
+  rr in H. des. rr in H0. des. rr. ss. esplits; et.
   2: { congruence. }
   eapply Forall2_app.
   - eapply Forall2_apply_Forall2; et. ii; ss. des_ifs. ss. des; clarify. esplits; et.
     ii. unfold focus_left. rewrite H4. refl.
   - eapply Forall2_apply_Forall2; et. ii; ss. des_ifs. ss. des; clarify. esplits; et.
     ii. unfold focus_right. rewrite H4. refl.
+Qed.
+
+Global Program Instance ModSem_equiv_ref: subrelation ((≡)) (⊑).
+Next Obligation.
+  r; i. eapply ModSemPair.adequacy.
+  destruct x as [x|].
+  2: { upt. des_ifs. }
+  destruct y as [y|].
+  2: { upt. des_ifs. }
+  upt. ss. destruct H as [T U].
+  econs; ss.
+  { instantiate (1:=top2). ss. }
+  2: { instantiate (2:=unit).
+       instantiate (1:=fun _ '(st_src, st_tgt) => st_src = st_tgt). ss. }
+  i. ss.
+  eapply Forall2_In_r in FINDS; et. des. des_ifs. des; ss. clarify.
+  esplits; et.
+  admit "ez - eutt".
+Qed.
+
+Global Program Instance ModSem_ref_refB: subrelation (⊑) ((⊑B)).
+Next Obligation.
+  do 1 r. i. do 2 r in H. specialize H with mytt. upt. des_ifs.
+Qed.
+
+Global Program Instance ModSem_RefBFacts: RefBFacts.
+Next Obligation.
+  econs.
+  - ii; ss.
+  - ii. eapply H0. eapply H; ss.
+Qed.
+Next Obligation.
+  etrans; typeclasses eauto.
 Qed.
 
 Global Program Instance ModSem_Ref_PreOrder: PreOrder ((⊑)).
@@ -86,13 +131,16 @@ Next Obligation.
   ii. eapply H0. eapply H; ss.
 Qed.
 
-(* Global Program Instance ModSem_EpsFacts: EpsFacts. *)
-(* Next Obligation. *)
-(*   ii; ss. *)
-(* Qed. *)
-(* Next Obligation. *)
-(*   ii. eapply H0. eapply H; ss. *)
-(* Qed. *)
+Global Program Instance ModSem_EpsFacts: EpsFacts.
+Next Obligation.
+  upt. des_ifs. refl.
+Qed.
+Next Obligation.
+  upt. des_ifs. refl.
+Qed.
+Next Obligation.
+  upt. des_ifs.
+Qed.
 
 (*
 a ⊑ a'
@@ -120,15 +168,30 @@ TTTTTTTTTTTTTTTTTTTTTTTTTTTTTTTTTTTTTTTTTTTTTTTTTTTTTTTTTTTTTTTTTTTTTTTttt
 Global Program Instance ModSem_RefFacts: RefFacts (T:=ModSem.t).
 Next Obligation.
   do 3 r. i.
-  {
-    ii.
-    eapply oplus_assoc_weak.
-  }
-  
-  rewrite oplus_assoc_weak.
-  rewrite H.
-  - ii; ss.
-  - ii. eapply H0. eapply H; ss.
+  unfold ref, ModSem.ref in *.
+  i. rewrite oplus_assoc_weak. rewrite H0.
+  rewrite oplus_comm_weak. rewrite oplus_assoc_weak. rewrite H.
+  rewrite oplus_assoc_weak2. rewrite oplus_comm_weak.
+  rewrite oplus_assoc_weak2. refl.
+Qed.
+
+Global Program Instance ModSem_MRA: MRA.t := {
+  car := ModSem.t;
+}.
+Next Obligation.
+  econs.
+  - ii. upt. des_ifs; try refl.
+  - ii. upt. des_ifs; try sym; et.
+  - ii. upt. des_ifs; etrans; et.
+Qed.
+Next Obligation.
+  econs.
+  - i. upt. des_ifs.
+    + eapply equiv_ref_both. erewrite ModSem.core_idemp.
+      r. esplits.
+      { erewrite ModSem.core_idemp. ii. upt. des_ifs; try refl.
+  - ii. upt. des_ifs; try sym; et.
+  - ii. upt. des_ifs; etrans; et.
 Qed.
 
 End FACTS.
